compiler/backend/bvl_to_bviScript.sml
@@ -215,6 +215,11 @@ local val compile_op_quotation = `
                [Op (Const 0) [];
                 Call 0 (SOME SumListLength_location)
                   [Var 0; Op (Const 0) []] NONE]] NONE)
+    | CopyByte T => (* TODO: this should eventually be implemented in data_to_word instead for efficiency *)
+      Let (if LENGTH c1 < 3 then (c1 ++ REPLICATE 3 (Op (Const 0) [])) else c1)
+        (Let [Op (RefByte T) [Op (Const 0) []; Var 0]]
+           (Let [Op (CopyByte F) [Op (Const 0) []; Var 0; Var 1; Var 2; Var 3]]
+             (Var 1)))
     | _ => Op op c1`
 in
 val compile_op_def = Define compile_op_quotation
